lemma/path_assoc.v
@@ -1,0 +1,496 @@
+(* From mathcomp Require Import ssreflect.seq all_ssreflect. *)
+From Paco Require Import paco pacotac.
+From SST Require Import src.expr src.header src.local CpdtTactics src.lcontext.
+From SST Require Import src.global src.projection src.part  src.balanced src.merge src.wfltt src.gttreeh.
+From SST Require Import lemma.projection lemma.projection_helper lemma.decidable lemma.liveness_helpers lemma.soundness.
+From SST Require Import src.step lemma.step src.assoc lemma.completeness  src.ltth src.path_props.
+Require Import List String Coq.Arith.PeanoNat Morphisms Relations Setoid.
+Require Import Coq.Program.Equality.
+Require Import Coq.Init.Logic.
+
+Lemma eventually_if {A:Type}: 
+forall (P Q : coseq A -> Prop) (xs:coseq A), eventually P xs -> 
+(forall ys, P ys -> eventually Q ys) -> eventually Q xs.
+Proof.
+    intros.
+    induction H;[crush|].
+
+    constructor 2. easy.
+Qed.
+
+
+Definition xs_height_map_fn := fun u : option (sort * gtth) =>
+match u with
+| Some (_, x) => gtth_height x
+| None => 0
+end.
+
+Lemma gtth_height_fold : forall p q xs, 
+gtth_height (gtth_send p q xs) =
+seq.foldr ( fun g a => Init.Nat.max (xs_height_map_fn g + 1) a) 1 xs.
+Proof.
+    intros * .
+    induction xs.
+    { 
+        simpl;easy.   
+    }
+    {
+        destruct a. 
+        destruct p0. rewrite gtth_height_unfold_once_some.
+        simpl seq.foldr. rewrite IHxs;easy.
+        rewrite gtth_height_unfold_once_none. simpl seq.foldr.
+        rewrite <- IHxs.
+        rewrite Nat.max_0_l.
+        
+        destruct (gtth_height (gtth_send p q xs)) eqn:Hyg;try easy.
+        eapply gtth_height_0_means_hol_general in Hyg;destr_hyps;easy.
+    }
+Qed.
+
+
+Variant coseq_bisimI {A:Type} (R: coseq A -> coseq A -> Prop): 
+coseq A -> coseq A -> Prop :=
+    | coseq_bis_nil : coseq_bisimI R conil conil
+    | coseq_bis_cons: forall xs ys x y, 
+    R xs ys -> coseq_bisimI R (cocons x xs) (cocons y ys).
+
+Definition coseq_bisimC {A:Type}:= paco2 ( @coseq_bisimI A) bot2.
+
+
+
+Variant path_assoc (R:local_path -> global_path -> Prop): local_path -> global_path -> Prop :=
+   | path_assoc_nil : path_assoc R conil conil
+   | path_assoc_xs : forall g gamma l xs ys, assoc gamma g ->
+    R xs ys ->
+   path_assoc R (cocons (gamma, l) xs) (cocons (g, l) ys)
+   .
+
+Lemma path_assoc_mon : monotone2 path_assoc.
+Proof. red;intros. inversion IN;subst;constructor;try tauto. apply LE;easy. Qed.
+   
+Definition path_assocC := paco2 path_assoc bot2.
+
+Definition conj_props (P:tctx -> Prop) (Q: gtt -> Prop) := forall gamma g,
+
+assoc gamma g -> (P gamma <-> Q g).
+
+Definition tctxREN_comm p q g := exists n, (tctxRE (lcomm p q n) g). 
+
+
+Definition tctxREN_send p q g := exists n s, (tctxRE (lsend p q s n) g).
+
+Definition tctxREN_recv p q g := exists n s, (tctxRE (lrecv p q s n) g).
+
+Print alwaysG.
+
+Definition wfg_global_path := alwaysCG (to_path_prop (fun a=> wfgC a /\ projectableA a) True).
+Definition wf_local_path := alwaysCG (to_path_prop tctx_wf True).
+Lemma global_path_always_wf : forall g l xs, wfgC g -> projectableA g -> global_valid_pathC (cocons (g,l) xs) -> 
+wfg_global_path (cocons (g,l) xs).
+Proof.
+    pcofix CIH.
+    intros * Hwfg Hprojable Hvalid.
+    pfold. constructor. simpl;easy.
+    destruct xs. left. pfold. constructor. easy.
+    right. destruct p.  pinversion Hvalid;subst;try apply valid_path_mon;try easy.
+    eapply CIH;
+    
+    red in H5; destruct l0;try tauto.
+    inversion Hvalid;subst.
+    eapply wfgC_after_step;try exact H5;try easy. eapply projectable_after_step;try exact H5;try easy.
+Qed.
+
+
+Lemma local_path_always_wf : forall g l xs, tctx_wf g -> local_valid_pathC (cocons (g,l) xs) -> 
+wf_local_path (cocons (g,l) xs).
+Proof.
+    pcofix CIH.
+    intros * Hwfg  Hvalid.
+    pfold. constructor. simpl;easy.
+    destruct xs. left. pfold. constructor. easy.
+    right. destruct p.  pinversion Hvalid;subst;try apply valid_path_mon;try easy.
+    eapply CIH;
+    
+    red in H5; destruct l0;try tauto.
+    inversion Hvalid;subst.
+    eapply tctx_wf_after_red_comm;try exact H5;try easy.
+Qed.
+
+Lemma eventually_and {A:Type} P Q : forall (xs:coseq A),
+            eventually ( P /1\ Q) xs <-> eventually (Q /1\ P) xs.
+            Proof. split;intros; induction H; 
+            try solve [constructor; easy | constructor 2; easy].  Qed.
+            
+Lemma path_assoc_eventually_enabled : forall xs ys P Q, wfg_global_path ys -> wf_local_path xs -> path_assocC xs ys -> 
+conj_props P Q -> eventually (to_path_prop  P False) xs -> eventually (to_path_prop  Q False) ys.
+Proof.
+    intros * Hwfgp Hwfgl Hpassoc Hconj Hevp.
+    generalize dependent ys.
+    induction Hevp.
+    {
+        intros. constructor. red in H. destruct xs;try easy.
+        pinversion Hpassoc;try apply path_assoc_mon;subst.
+        red.
+        eapply Hconj with (gamma:=gamma); easy. 
+    }
+    {
+     intros.
+     pinversion Hpassoc;try apply path_assoc_mon;subst.
+     constructor 2.
+     eapply IHHevp.
+     pinversion Hwfgl;try apply always_mon;subst;easy.
+     pinversion Hwfgp;try apply always_mon;subst;easy.
+     easy.   
+    }
+Qed.
+Lemma path_assoc_preserves_fairness_helper : forall xs p q ys, path_assocC xs ys ->
+eventually (headComm p q) xs -> eventually (headComm_global p q) ys.
+Proof.
+    intros * Hpassoc Hevp.
+    generalize dependent ys. induction Hevp.
+    {
+        intros. red in H. destruct xs as [ | [t l]];try easy.
+        destruct l;try tauto;destruct l;try tauto.
+        destruct (Nat.eq_dec p n);destruct (Nat.eq_dec q n0);try tauto;subst;clear H.
+        pinversion Hpassoc;try apply path_assoc_mon;subst. constructor.  simpl. tauto.
+    }
+    {
+        intros * Hpassoc. pinversion Hpassoc;try apply path_assoc_mon;subst.
+        constructor 2.
+        eapply IHHevp. easy.  
+    }
+Qed.
+
+
+Lemma global_comm_enabled_assoc_local_comm_enabled: forall p q n gamma g, wfgC g ->
+tctx_wf gamma -> global_comm_enabled p q n g -> 
+assoc gamma g -> exists n', tctxRE (lcomm p q n') gamma.
+Proof.
+    intros * Hwfg Hwft Hgce Hassoc. 
+    red in Hgce. destr_hyps. eapply assoc_soundness with (gamma:=gamma) in H;try easy.
+    destr_hyps. exists x2. red. exists x0;easy.
+    pinversion H;subst;try apply step_mon;easy.
+Qed.
+
+Lemma wfg_global_path_head: forall g l ys, wfg_global_path (cocons (g,l) ys) -> wfgC g.
+Proof.
+    intros. pinversion H;try apply always_mon;subst. red in H2. tauto.
+Qed.
+
+Lemma projable_global_path_head: forall g l ys, wfg_global_path (cocons (g,l) ys) -> projectableA g.
+Proof.
+    intros. pinversion H;try apply always_mon;subst. red in H2. tauto.
+Qed.
+
+Lemma wf_local_path_head: forall g l ys, wf_local_path (cocons (g,l) ys) -> tctx_wf g.
+Proof.
+    intros. pinversion H;try apply always_mon;subst. red in H2. tauto.
+Qed.
+
+Lemma always_tail {A:Type}: forall (g:A) (l:option label) xs P, alwaysCG P (cocons (g,l) xs) -> alwaysCG P xs.
+Proof. intros. pinversion H;try apply always_mon;subst. easy. Qed.
+
+
+    
+Lemma path_assoc_preserves_fairness : forall lp gp, wfg_global_path gp -> wf_local_path lp ->
+path_assocC lp gp ->
+fair_path lp -> fair_path_global gp.
+Proof.
+    pcofix CIH.
+    intros * Hwfgp Hwflp Hpassoc Hfairl.
+    pfold.
+    pinversion Hpassoc;try apply path_assoc_mon;subst.
+    {
+        constructor. red. intros. simpl in H. easy.
+    }
+    constructor.
+    { 
+        red. intros.
+        pinversion Hfairl;subst;try apply always_mon.
+        red in H4.
+        simpl in H1.
+        
+        eapply global_comm_enabled_assoc_local_comm_enabled in H1 as Hlc;try exact Hassoc;try easy;
+        try solve [
+        apply wfg_global_path_head in Hwfgp;easy | apply wf_local_path_head in Hwflp;easy].
+        destruct Hlc as [n' Hr].
+        
+        specialize (H4 p q n').
+        simpl in H4. 
+        specialize (H4 Hr). inversion H4;subst.
+        {  
+            simpl in H2.
+            destruct l;try tauto.
+            destruct l; destruct (Nat.eq_dec p n0);destruct (Nat.eq_dec q n1);subst;try tauto.
+            constructor 1. simpl. tauto.
+        }
+        {
+            constructor 2. eapply path_assoc_preserves_fairness_helper;try exact H3;try easy.
+        }   
+    }
+    {
+        right. eapply CIH with (lp := xs);
+        eapply always_tail in Hwfgp, Hwflp, Hfairl;try easy.
+    }
+Qed.
+
+Lemma local_send_enabled_global_send_enabled : forall g p q s n gamma, wfgC g -> tctx_wf gamma ->
+        assoc gamma g -> tctxRE (lsend p q (Some s) n) gamma ->
+        exists s' n', global_label_enabled (lsend p q (Some s') n') g.
+Proof.
+    intros * Hwfg Hwf Hassoc Hre.
+    destruct Hre as [t' Hre].
+    eapply lem_6_11a_tctx_send_invert in Hre. destr_hyps. 
+    
+    eapply assoc_inv_find in H as Hinvf;try exact Hassoc;try easy.
+    red in Hinvf. destr_hyps. eapply subtype_send_inv1 in H3 as Hst. destr_hyps;subst. 
+    eapply subtype_send_inv in H3. eapply Forall2R_prop in H3;try exact H0;tac_sanitize.
+    exists x4, n.
+    red. exists x2, x6. tauto.
+Qed.
+
+Lemma local_recv_enabled_global_recv_enabled : forall g p q s n gamma, wfgC g -> tctx_wf gamma ->
+    assoc gamma g -> tctxRE (lrecv p q (Some s) n) gamma ->
+    exists s' n', global_label_enabled (lrecv p q (Some s') n') g.
+Proof.
+    intros * Hwfg Hwf Hassoc Hre.
+    destruct Hre as [t' Hre].
+    eapply lem_6_11b_tctx_recv_invert in Hre. destr_hyps. 
+    
+    eapply assoc_inv_find in H as Hinvf;try exact Hassoc;try easy.
+    red in Hinvf. destr_hyps. eapply subtype_recv_inv1 in H3 as Hst. destr_hyps;subst.
+    
+    eapply projection_implies_wf in H2 as Hwfp;try easy.
+    eapply wfltt_slist_recv in Hwfp as Hslist. eapply slist_implies_some in Hslist.
+    destr_hyps. destruct x3. exists s0,x1.
+    red. exists x2, l. tauto.
+Qed.
+
+Lemma path_assoc_reflects_liveness_helper : forall xs p q ys, path_assocC xs ys ->
+eventually (headComm_global p q) ys -> eventually (headComm p q) xs.
+Proof.
+    intros * Hpassoc Hevp.
+    generalize dependent xs. induction Hevp.
+    {
+        intros. red in H. destruct xs as [ | [t l]];try easy.
+        destruct l;try tauto;destruct l;try tauto.
+        destruct (Nat.eq_dec p n) ;destruct (Nat.eq_dec q n0);try tauto;subst;clear H.
+        pinversion Hpassoc;try apply path_assoc_mon;subst. constructor. simpl. tauto.
+    }
+    {
+        intros * Hpassoc. pinversion Hpassoc;try apply path_assoc_mon;subst.
+        constructor 2.
+        eapply IHHevp. easy.  
+    }
+Qed.
+
+Lemma path_assoc_reflects_liveness : forall lp gp, wfg_global_path gp -> wf_local_path lp ->
+path_assocC lp gp ->
+live_path_global gp -> live_path lp.
+Proof.
+    pcofix CIH.
+    intros * Hwfgp Hwflp Hpassoc Hfairl.
+    pfold.
+    pinversion Hpassoc;try apply path_assoc_mon;subst.
+    {
+        constructor. red;split; intros; simpl in H; easy.
+    }
+    constructor.
+    { 
+        red;split; intros;
+        pinversion Hfairl;subst;try apply always_mon;
+        red in H4;
+        simpl in H1;
+
+        [eapply local_send_enabled_global_send_enabled in H1 as Hlc 
+        | eapply local_recv_enabled_global_recv_enabled in H1 as Hlc];
+        try exact Hassoc;try easy;
+        try solve [
+        apply wfg_global_path_head in Hwfgp;easy | apply wf_local_path_head in Hwflp;easy];
+        destruct Hlc as [s' [n' Hr]];
+        
+        specialize (H4 p q s' n'); destruct H4 as [Hlv1 Hlv2];
+        [
+        assert(Hevg: eventually (headComm_global p q) (cocons (g,l) ys)) by (eapply Hlv1;easy)
+        |
+        assert(Hevg: eventually (headComm_global p q) (cocons (g,l) ys)) by (eapply Hlv2;easy)];
+        eapply path_assoc_reflects_liveness_helper with (ys:=(cocons (g,l) ys));try easy;
+        pfold;easy.
+    }
+    {
+        right. eapply CIH with (gp := ys);
+        eapply always_tail in Hwfgp, Hwflp, Hfairl;try easy.
+    }
+Qed.
+
+(*
+Definition g_by_gamma_trans : forall t p q ell g t', wfgC g -> tctx_wf t -> assoc t g ->
+tctxR t (lcomm p q ell) t' ->
+{g' | assoc t' g' /\ gttstepC g g' p q ell}.
+Proof.
+    intros. eapply assoc_completeness with (g:=g) in H0;try exact H2;try easy.
+    destruct (constructive_indefinite_description _ H0) as [g' Hg'].
+    exists g'. easy.
+Defined.
+
+
+Lemma valid_local_path_valid_trans: forall t p q ell xs,
+valid_local_path (cocons (t, Some (lcomm p q ell)) xs) ->
+{s| match s with (t',l,ys) => 
+xs= cocons (t',l) ys /\ tctxR t (lcomm p q ell) t' end}.
+Proof.
+    intros. 
+    refine (
+        (match xs as m return xs =m -> {s| match s with (t',l,ys) => 
+xs= cocons (t',l) ys /\ tctxR t (lcomm p q ell) t' end} with 
+    |conil => _
+    | cocons (t',l) ys => _ end
+) (eq_refl)).
+    {
+        intros. subst.
+        assert(False).
+        {
+            pinversion H;try apply valid_path_mon.   
+        }
+        exists (M.empty, None, conil). easy.   
+    }
+    {
+        intros. subst. exists (t', l, ys).
+        split. easy.
+        pinversion H;subst;try apply valid_path_mon. easy.   
+    }
+Defined.
+
+
+Lemma valid_local_path_dilemma: forall t l xs, valid_local_path (cocons (t,l) xs) ->
+{ s & match s with (p,q,ell) => {l=Some (lcomm p q ell)} + {l=None} end }.
+Proof.
+    intros.
+    destruct l;try tauto.
+    {
+        assert(Hrec: { s | match s with (p,q,ell) => l=lcomm p q ell end}).
+        {
+                refine ((match l as m return 
+                (l=m -> { s | match s with (p,q,ell) => l=lcomm p q ell end}) with 
+                | lsend a b c d => _
+                | lrecv a b c d => _
+                
+                | lcomm p q ell => _ end) (eq_refl));intros;subst;
+                try (
+                assert(False) by
+                (
+                    pinversion H;subst;try apply valid_path_mon; inversion H4  
+                );
+                exists (0,0,0); easy).
+                exists (p,q,ell). reflexivity.
+        }
+        destruct Hrec. destruct x as [[p q] ell]. subst. exists (p,q,ell). tauto.
+    }
+    {
+        exists (0,0,0). right. easy.   
+    }
+Defined.
+(*
+Ltac indef_destruct H := let tth := type of H in match tth with 
+     | ex _  => let nx := fresh "x" in let nh:= fresh "H" in  
+    destruct (constructive_indefinite_description _ H) as [nx nh];try indef_destruct nh;clear H end.
+*)   
+CoFixpoint conj_path : forall t g l  xs, wfgC g -> tctx_wf t -> assoc t g ->
+    valid_local_path (cocons (t, l) xs) ->
+    global_path.
+Proof.
+    intros * Hwfg Htxt Hassoc Hvalid.
+    eapply valid_local_path_dilemma in Hvalid as Hdl.
+    destruct Hdl as [[[p q] ell] Hdd].
+    destruct Hdd.
+    {
+        subst.
+        eapply valid_local_path_valid_trans in Hvalid as Htrans.
+        destruct Htrans as [[[t' l] ys] H1].
+        
+        destruct H1;subst. 
+        set (seq_hd := (g,Some (lcomm p q ell))).
+        eapply g_by_gamma_trans with (g:=g) in H0 as Ht2;try easy.
+        destruct Ht2.
+        rename  x into g'.
+        destruct a as [Ha0 Ha1].
+        assert(Hwft': tctx_wf t').
+        {
+            eapply tctx_wf_after_red_comm;try exact H0;try easy.   
+        }
+        assert(Hwfg': wfgC g').
+        {
+
+            eapply wfgC_after_step;try exact Ha1;try easy.
+            eapply assoc_implies_projectable;try exact Hassoc;try easy.   
+        }
+        assert(Hvlxs: valid_local_path (cocons (t', l) ys)).
+        {
+            pinversion Hvalid;try apply valid_path_mon;tauto.   
+        }
+        
+        specialize (conj_path t' g' l ys Hwfg' Hwft' Ha0 Hvlxs) as vxs.
+        exact (cocons seq_hd vxs).
+    }
+    subst. exact (cocons (g, None) conil).
+Defined.
+
+
+Lemma conj_path_recur : forall (t:tctx) (g:gtt) (l:option label) (xs:local_path) 
+ (Hwfg : wfgC g) (Htxwf : tctx_wf t) (Hassoc: assoc t g) 
+(Hvalid : valid_local_path (cocons (t,l) xs)), exists ys,
+(conj_path _ _ _ _ Hwfg Htxwf Hassoc Hvalid) = cocons (g,l) ys.
+Proof.
+    intros.
+    destruct l.
+    {
+           destruct l;
+        pose proof Hvalid as Hvalid'; pinversion Hvalid'; try apply valid_path_mon;try tauto;subst.
+        rewrite (coseq_eq (conj_path _ _ _ _ _ _ _ _   )). simpl.
+
+        destruct (g_by_gamma_trans t n n0 n1 g x Hwfg Htxwf Hassoc) (eqn:Hyg).
+        Check eq_rec_r.
+
+    }
+    {
+        rewrite (coseq_eq (conj_path _ _ _ _ _ _ _ _   )). simpl. exists conil;easy.
+    }
+    
+
+Lemma conj_path_path_assoc : forall (t:tctx) (g:gtt) (l:option label) (xs:local_path) 
+ (Hwfg : wfgC g) (Htxwf : tctx_wf t) (Hassoc: assoc t g) 
+(Hvalid : valid_local_path (cocons (t,l) xs)),
+
+path_assocC (cocons (t,l) xs) 
+(conj_path _ _ _ _ Hwfg Htxwf Hassoc Hvalid).
+Proof.
+    pcofix CIH.
+    intros.
+    destruct l.
+    {
+        destruct l;
+        pose proof Hvalid as Hvalid'; pinversion Hvalid'; try apply valid_path_mon;try tauto;subst.
+
+        rewrite (coseq_eq (conj_path _ _ _ _ _ _ _ _   )).
+        pfold.
+           
+            
+    }
+    {
+        Search valid_path_GC conil.
+        eapply valid_path_none_next_nil in Hvalid as Hv2;subst.
+        pfold.
+        assert(conj_path t g None conil Hwfg Htxwf Hassoc Hvalid = cocons (g,None) conil).
+        {
+            rewrite (coseq_eq (conj_path _ _ _ _ _ _ _ _   )).
+            simpl. reflexivity.
+        }
+        rewrite H. constructor;try tauto.
+        left. pfold. constructor.     
+    }
+*)
+
+Lemma conj_path_exists: forall g gamma xs l, wfgC g -> tctx_wf gamma -> assoc gamma g ->
+    exists ys, path_assocC (cocons (gamma,l) xs) (cocons (g, l) ys).
+Proof.
+Admitted.
